Move principle_hnf stuff to solvableTheory

examples/lambda/barendregt/boehm_treeScript.sml
@@ -5,8 +5,8 @@
 open HolKernel boolLib Parse bossLib;
 
 (* core theories *)
-open optionTheory arithmeticTheory pred_setTheory listTheory llistTheory
-     relationTheory ltreeTheory pathTheory posetTheory hurdUtils;
+open optionTheory arithmeticTheory pred_setTheory listTheory rich_listTheory
+     llistTheory relationTheory ltreeTheory pathTheory posetTheory hurdUtils;
 
 open basic_swapTheory binderLib termTheory appFOLDLTheory chap2Theory
      chap3Theory head_reductionTheory standardisationTheory solvableTheory;
@@ -15,76 +15,6 @@ val _ = new_theory "boehm_tree";
 
 val _ = temp_delsimps ["lift_disj_eq", "lift_imp_disj"];
 val o_DEF = combinTheory.o_DEF; (* cannot directly open combinTheory *)
-
-(* Definition 8.3.20 [1, p.177]
-
-   A term may have several hnf's, e.g. if any of its hnf can still do beta
-   reductions, after such reductions the term is still an hnf by definition.
-   The (unique) terminating term of head reduction path is called "principle"
-   hnf, which is used for defining Boehm trees.
- *)
-Definition principle_hnf_def :
-    principle_hnf = last o head_reduction_path
-End
-
-Theorem hnf_principle_hnf :
-    !M. has_hnf M ==> hnf (principle_hnf M)
-Proof
-    rw [corollary11_4_8, principle_hnf_def]
- >> MP_TAC (Q.SPEC ‘M’ head_reduction_path_def)
- >> RW_TAC std_ss []
-QED
-
-Theorem principle_hnf_stable :
-    !M. hnf M ==> principle_hnf M = M
-Proof
-    rw [principle_hnf_def]
- >> ‘finite (head_reduction_path M)’ by PROVE_TAC [hnf_has_hnf, corollary11_4_8]
- >> MP_TAC (Q.SPEC ‘M’ head_reduction_path_def)
- >> RW_TAC std_ss []
- (* applying is_head_reduction_thm *)
- >> qabbrev_tac ‘p = head_reduction_path M’
- >> STRIP_ASSUME_TAC (ISPEC “p :(term, redpos list) path” path_cases)
- >- fs []
- >> gs [is_head_reduction_thm, hnf_no_head_redex]
-QED
-
-(* used by principle_hnf_LAMl_appstar *)
-Theorem lemma2[local] :
-    hnf t /\ (!y. MEM y (MAP SND pi) ==> y # t) ==>
-    principle_hnf (LAMl (MAP FST (REVERSE pi)) t @* MAP (VAR o SND) pi) = tpm pi t
-Proof
-    cheat
-QED
-
-(* ‘principle_hnf’ can be used to do final beta-reductions to make a hnf abs-free *)
-Theorem principle_hnf_LAMl_appstar :
-    !xs t vs pi. hnf t /\ vs = FRESH_list (LENGTH xs) (FV t) /\
-                 pi = ZIP (REVERSE xs,vs) ==>
-                 principle_hnf (LAMl xs t @* (MAP VAR vs)) = tpm pi t
-Proof
-    RW_TAC std_ss []
- >> qabbrev_tac ‘n = LENGTH xs’
- >> MP_TAC (Q.SPECL [‘n’, ‘FV (t :term)’] FRESH_list_def) >> rw []
- >> qabbrev_tac ‘vs = FRESH_list n (FV t)’
- >> qabbrev_tac ‘pi = ZIP (REVERSE xs,vs)’
- >> ‘LENGTH (REVERSE xs) = LENGTH vs’ by rw []
- >> ‘vs = MAP SND pi’ by rw [Abbr ‘pi’, MAP_ZIP]
- >> POP_ORW
- >> Know ‘REVERSE (REVERSE xs) = REVERSE (MAP FST pi)’
- >- rw [Abbr ‘pi’, MAP_ZIP]
- >> REWRITE_TAC [REVERSE_REVERSE, GSYM MAP_REVERSE]
- >> Rewr'
- >> simp [MAP_MAP_o]
- >> Know ‘!y. MEM y (MAP SND pi) ==> y # t’
- >- (Q.PAT_X_ASSUM ‘DISJOINT (set vs) (FV t)’ MP_TAC \\
-     rw [DISJOINT_ALT, Abbr ‘pi’, MEM_MAP, MEM_ZIP, MEM_EL] \\
-     simp [] \\
-     FIRST_X_ASSUM MATCH_MP_TAC \\
-     Q.EXISTS_TAC ‘n’ >> art [])
- >> DISCH_TAC
- >> MATCH_MP_TAC lemma2 >> rw []
-QED
 
 (* hnf_head access the head variable term of an abs-free hnf. *)
 local
